driver/PolOptBandTiling.v
@@ -77,6 +77,77 @@ Definition try_phase_pipeline_from_source_pol_band
       end
   end.
 
+Definition try_verified_diamond_after_phase_mid_band
+    (pol_mid: PolyLang.t)
+    (mid_scop posttile_scop after_scop: OpenScop): imp LoopIR.t :=
+  match BaseOpt.infer_tiling_witness_scops mid_scop posttile_scop with
+  | Err _ =>
+      PrepareCore.prepared_codegen pol_mid
+  | Okk ws =>
+      match ValidatorCore.import_canonical_tiled_after_poly pol_mid posttile_scop ws with
+      | Err _ =>
+          PrepareCore.prepared_codegen pol_mid
+      | Okk pol_posttile =>
+          BIND ok_shape <- TilingSched.checked_tiling_schedule_stripmined_validate_poly pol_mid pol_posttile ws -;
+          if ok_shape then
+            match TilingSched.infer_pprog_tiling_bands
+                    (TilingSched.Base.outer_to_tiling_pprog pol_mid) ws with
+            | None =>
+                PrepareCore.prepared_codegen pol_mid
+            | Some bands =>
+                BIND ok_perm <-
+                  TilingSched.check_pprog_permutable_tiling_bands_via_validate_tiling
+                    (TilingSched.Base.outer_to_tiling_pprog pol_mid)
+                    (TilingSched.Base.outer_to_tiling_pprog pol_posttile)
+                    ws bands -;
+                if ok_perm then
+                  BIND wf_posttile <- ValidatorCore.check_wf_polyprog_general pol_posttile -;
+                  if wf_posttile then
+                    match PolyLang.from_openscop_schedule_only pol_posttile after_scop with
+                    | Err _ =>
+                        PrepareCore.prepared_codegen pol_mid
+                    | Okk pol_after =>
+                        BIND final_ok <- ValidatorCore.validate_general pol_posttile pol_after -;
+                        if final_ok then
+                          BIND wf_after <- ValidatorCore.check_wf_polyprog_general pol_after -;
+                          if wf_after then
+                            PrepareCore.prepared_codegen
+                              (PolyLang.current_view_pprog pol_after)
+                          else
+                            PrepareCore.prepared_codegen pol_mid
+                        else
+                          PrepareCore.prepared_codegen pol_mid
+                    end
+                  else
+                    PrepareCore.prepared_codegen pol_mid
+                else
+                  PrepareCore.prepared_codegen pol_mid
+            end
+          else
+            PrepareCore.prepared_codegen pol_mid
+      end
+  end.
+
+Definition try_diamond_phase_pipeline_from_source_pol_band
+    (pol_source: PolyLang.t)
+    (before_scop: OpenScop): imp LoopIR.t :=
+  match BaseOpt.run_pluto_diamond_phase_pipeline before_scop with
+  | Err _ =>
+      BaseOpt.affine_only_opt_prepared_from_poly pol_source
+  | Okk (mid_scop, (posttile_scop, after_scop)) =>
+      match PolyLang.from_openscop_like_source pol_source mid_scop with
+      | Err _ =>
+          BaseOpt.affine_only_opt_prepared_from_poly pol_source
+      | Okk pol_mid =>
+          BIND affine_ok <- ValidatorCore.validate pol_source pol_mid -;
+          if affine_ok then
+            try_verified_diamond_after_phase_mid_band
+              pol_mid mid_scop posttile_scop after_scop
+          else
+            BaseOpt.affine_only_opt_prepared_from_poly pol_source
+      end
+  end.
+
 Definition phase_pipeline_opt_prepared_from_poly_no_iss_band
     (pol: PolyLang.t): imp LoopIR.t :=
   if BaseOpt.has_nonscalar_stmt pol then
@@ -92,11 +163,29 @@ Definition phase_pipeline_opt_prepared_from_poly_no_iss_band
   else
     PrepareCore.prepared_codegen pol.
 
+Definition phase_diamond_opt_prepared_from_poly_no_iss_band
+    (pol: PolyLang.t): imp LoopIR.t :=
+  if BaseOpt.has_nonscalar_stmt pol then
+    match BaseOpt.export_for_phase_scheduler pol with
+    | Some before_scop =>
+        try_diamond_phase_pipeline_from_source_pol_band pol before_scop
+    | None =>
+        BaseOpt.affine_only_opt_prepared_from_poly pol
+    end
+  else
+    PrepareCore.prepared_codegen pol.
+
 Definition phase_pipeline_opt_prepared_band
     (loop: LoopIR.t): imp LoopIR.t :=
   BIND pol0 <- res_to_alarm PolyLang.dummy (BaseOpt.Extractor.extractor loop) -;
   let pol := BaseOpt.Strengthen.strengthen_pprog pol0 in
   phase_pipeline_opt_prepared_from_poly_no_iss_band pol.
+
+Definition phase_diamond_opt_prepared_band
+    (loop: LoopIR.t): imp LoopIR.t :=
+  BIND pol0 <- res_to_alarm PolyLang.dummy (BaseOpt.Extractor.extractor loop) -;
+  let pol := BaseOpt.Strengthen.strengthen_pprog pol0 in
+  phase_diamond_opt_prepared_from_poly_no_iss_band pol.
 
 Lemma try_verified_tiling_after_phase_mid_band_correct:
   forall pol_mid mid_scop after_scop st st',
@@ -339,6 +428,304 @@ Proof.
   eapply State.eq_trans.
   - exact Heq_str.
   - exact Heq_src.
+Qed.
+
+Lemma try_verified_diamond_after_phase_mid_band_correct:
+  forall pol_mid mid_scop posttile_scop after_scop st st',
+    PolyLang.wf_pprog_affine pol_mid ->
+    WHEN loop' <-
+      try_verified_diamond_after_phase_mid_band
+        pol_mid mid_scop posttile_scop after_scop THEN
+    LoopIR.semantics loop' st st' ->
+    exists st'',
+      PolyLang.instance_list_semantics pol_mid st st'' /\
+      State.eq st' st''.
+Proof.
+  intros pol_mid mid_scop posttile_scop after_scop st st'
+         Hwf_mid loop' Hopt Hloop.
+  unfold try_verified_diamond_after_phase_mid_band in Hopt.
+  destruct (BaseOpt.infer_tiling_witness_scops mid_scop posttile_scop)
+    as [ws|msg] eqn:Hws.
+  - destruct
+      (ValidatorCore.import_canonical_tiled_after_poly pol_mid posttile_scop ws)
+      as [pol_posttile|msg_after] eqn:Hposttile.
+    + bind_imp_destruct Hopt ok_shape Hcheck_shape.
+      destruct ok_shape.
+      * destruct (TilingSched.infer_pprog_tiling_bands
+                    (TilingSched.Base.outer_to_tiling_pprog pol_mid) ws)
+          as [bands|] eqn:Hbands.
+        -- bind_imp_destruct Hopt ok_perm Hcheck_perm.
+           destruct ok_perm.
+           ++ bind_imp_destruct Hopt wf_posttile_ok Hwf_posttile_check.
+              destruct wf_posttile_ok.
+              ** destruct (PolyLang.from_openscop_schedule_only
+                             pol_posttile after_scop)
+                   as [pol_after|msg_final] eqn:Hafter.
+                 --- bind_imp_destruct Hopt final_ok Hfinal.
+                     destruct final_ok.
+                     +++ bind_imp_destruct Hopt wf_after_ok Hwf_check.
+                         destruct wf_after_ok.
+                         *** pose proof
+                           (ValidatorCore.check_wf_polyprog_general_correct
+                              pol_after true Hwf_check eq_refl)
+                           as Hwf_after.
+                         pose proof
+                           (PrepareCore.prepared_codegen_correct_general
+                              pol_after st st' loop' Hopt Hwf_after Hloop)
+                           as Hsem_after.
+                         pose proof
+                           (ValidatorCore.validate_general_correct
+                              pol_posttile pol_after st st'
+                              true Hfinal eq_refl Hsem_after)
+                           as Hfinal_corr.
+                         destruct Hfinal_corr as [st_post [Hpost_sem Heq_post]].
+                         remember (TilingSched.Base.outer_to_tiling_pprog pol_mid)
+                           as before_tiling eqn:Hbefore_tiling_eq.
+                         remember (TilingSched.Base.outer_to_tiling_pprog pol_posttile)
+                           as after_tiling eqn:Hafter_tiling_eq.
+                         pose proof Hcheck_shape as Hcheck_shape_sched.
+                         unfold TilingSched.checked_tiling_schedule_stripmined_validate_poly,
+                                TilingSched.checked_tiling_schedule_stripmined_validate_outer
+                           in Hcheck_shape.
+                         unfold TilingSched.checked_tiling_schedule_stripmined_validate_poly,
+                                TilingSched.checked_tiling_schedule_stripmined_validate_outer,
+                                TilingSched.checked_tiling_schedule_stripmined_validate
+                           in Hcheck_shape_sched.
+                         apply mayReturn_pure in Hcheck_shape_sched.
+                         apply andb_true_iff in Hcheck_shape_sched.
+                         destruct Hcheck_shape_sched as [_ Hsched_only].
+                         destruct before_tiling as [[before_pis before_ctxt] before_vars].
+                         destruct after_tiling as [[after_pis after_ctxt] after_vars].
+                         simpl in Hbefore_tiling_eq, Hafter_tiling_eq.
+                         rewrite <- Hbefore_tiling_eq in Hcheck_shape, Hsched_only.
+                         rewrite <- Hafter_tiling_eq in Hcheck_shape, Hsched_only.
+                         simpl in Hcheck_shape, Hsched_only, Hbands.
+                         pose proof
+                           (TilingSched.check_pprog_tiling_schedule_stripminedb_ctxt_sound
+                              (before_pis, before_ctxt, before_vars)
+                              (after_pis, after_ctxt, after_vars)
+                              ws Hsched_only)
+                           as [Hctxt_eq Hvars_eq].
+                         pose proof
+                           (TilingSched.Base.outer_to_tiling_wf_pprog_affine
+                              pol_mid Hwf_mid)
+                           as Hwf_before_tiling.
+                         rewrite <- Hbefore_tiling_eq in Hwf_before_tiling.
+                         destruct Hwf_before_tiling as [_ Hwf_before_tiling].
+                         assert (Hwfbefore_pis :
+                           List.Forall
+                             (TilingSched.Base.Tiling.PL.wf_pinstr_tiling
+                                before_ctxt before_vars)
+                             before_pis).
+                         {
+                           eapply List.Forall_forall.
+                           intros pi Hin.
+                           eapply
+                             TilingSched.Base.Tiling.PL.wf_pinstr_affine_implies_wf_pinstr_tiling.
+                           eapply Hwf_before_tiling; eauto.
+                         }
+                         pose proof
+                           (ValidatorCore.check_wf_polyprog_general_correct
+                              pol_posttile true Hwf_posttile_check eq_refl)
+                           as Hwf_posttile.
+                         pose proof
+                           (TilingSched.Base.outer_to_tiling_wf_pprog_general
+                              pol_posttile Hwf_posttile)
+                           as Hwf_after_tiling.
+                         rewrite <- Hafter_tiling_eq in Hwf_after_tiling.
+                         rewrite <- Hctxt_eq, <- Hvars_eq in Hwf_after_tiling.
+                         destruct Hwf_after_tiling as [_ Hwf_after_tiling].
+                         assert (Hwfafter_pis :
+                           List.Forall
+                             (TilingSched.Base.Tiling.PL.wf_pinstr_tiling
+                                before_ctxt before_vars)
+                             after_pis).
+                         {
+                           eapply List.Forall_forall.
+                           intros pi Hin.
+                           eapply Hwf_after_tiling; eauto.
+                         }
+                         rewrite <- Hctxt_eq, <- Hvars_eq in Hcheck_shape, Hcheck_perm.
+                         pose proof
+                           (TilingSched.checked_tiling_schedule_stripmined_and_band_validate_correct_same_ctxt
+                              before_pis before_ctxt before_vars
+                              after_pis
+                              ws bands st st_post
+                              Hcheck_shape Hbands
+                              Hwfbefore_pis Hwfafter_pis
+                              Hcheck_perm)
+                           as Hcorr.
+                         apply TilingSched.Base.outer_to_tiling_instance_list_semantics_iff
+                           in Hpost_sem.
+                         rewrite <- Hafter_tiling_eq in Hpost_sem.
+                         rewrite <- Hctxt_eq, <- Hvars_eq in Hpost_sem.
+                         specialize (Hcorr Hpost_sem).
+                         destruct Hcorr as [st_mid [Hmid_tiling Heq_mid]].
+                         rewrite Hbefore_tiling_eq in Hmid_tiling.
+                         apply TilingSched.Base.outer_to_tiling_instance_list_semantics_iff
+                           in Hmid_tiling.
+                         exists st_mid.
+                         split; auto.
+                         eapply State.eq_trans; eauto.
+                         *** pose proof
+                           (PrepareCore.prepared_codegen_correct
+                              pol_mid st st' loop' Hopt Hwf_mid Hloop)
+                           as Hmid_sem.
+                         exists st'. split; auto. apply State.eq_refl.
+                     +++ pose proof
+                       (PrepareCore.prepared_codegen_correct
+                          pol_mid st st' loop' Hopt Hwf_mid Hloop)
+                       as Hmid_sem.
+                     exists st'. split; auto. apply State.eq_refl.
+                 --- pose proof
+                   (PrepareCore.prepared_codegen_correct
+                      pol_mid st st' loop' Hopt Hwf_mid Hloop)
+                   as Hmid_sem.
+                 exists st'. split; auto. apply State.eq_refl.
+              ** pose proof
+                   (PrepareCore.prepared_codegen_correct
+                      pol_mid st st' loop' Hopt Hwf_mid Hloop)
+                   as Hmid_sem.
+                 exists st'. split; auto. apply State.eq_refl.
+           ++ pose proof
+                (PrepareCore.prepared_codegen_correct
+                   pol_mid st st' loop' Hopt Hwf_mid Hloop)
+                as Hmid_sem.
+              exists st'. split; auto. apply State.eq_refl.
+        -- pose proof
+             (PrepareCore.prepared_codegen_correct
+                pol_mid st st' loop' Hopt Hwf_mid Hloop)
+             as Hmid_sem.
+           exists st'. split; auto. apply State.eq_refl.
+      * pose proof
+           (PrepareCore.prepared_codegen_correct
+              pol_mid st st' loop' Hopt Hwf_mid Hloop)
+          as Hmid_sem.
+        exists st'. split; auto. apply State.eq_refl.
+    + pose proof
+         (PrepareCore.prepared_codegen_correct
+            pol_mid st st' loop' Hopt Hwf_mid Hloop)
+        as Hmid_sem.
+      exists st'. split; auto. apply State.eq_refl.
+  - pose proof
+       (PrepareCore.prepared_codegen_correct
+          pol_mid st st' loop' Hopt Hwf_mid Hloop)
+      as Hmid_sem.
+    exists st'. split; auto. apply State.eq_refl.
+Qed.
+
+Lemma try_diamond_phase_pipeline_from_source_pol_band_correct:
+  forall pol_source before_scop st st',
+    PolyLang.wf_pprog_affine pol_source ->
+    WHEN loop' <-
+      try_diamond_phase_pipeline_from_source_pol_band
+        pol_source before_scop THEN
+    LoopIR.semantics loop' st st' ->
+    exists st'',
+      PolyLang.instance_list_semantics pol_source st st'' /\
+      State.eq st' st''.
+Proof.
+  intros pol_source before_scop st st' Hwf_source loop' Hopt Hloop.
+  unfold try_diamond_phase_pipeline_from_source_pol_band in Hopt.
+  destruct (BaseOpt.run_pluto_diamond_phase_pipeline before_scop)
+    as [[mid_scop [posttile_scop after_scop]]|msg] eqn:Hphase.
+  - destruct (PolyLang.from_openscop_like_source pol_source mid_scop)
+      as [pol_mid|msg_mid] eqn:Hmid.
+    + bind_imp_destruct Hopt affine_ok Haff.
+      destruct affine_ok.
+      * pose proof
+          (ValidatorCore.validate_preserve_wf_pprog
+             pol_source pol_mid _ Haff eq_refl)
+          as [_ Hwf_mid].
+        pose proof
+          (try_verified_diamond_after_phase_mid_band_correct
+             pol_mid mid_scop posttile_scop after_scop
+             st st' Hwf_mid loop' Hopt Hloop)
+          as Hmid_corr.
+        destruct Hmid_corr as [st_mid [Hmid_sem Heq_mid]].
+        pose proof
+          (ValidatorCore.validate_correct
+             pol_source pol_mid st st_mid true Haff eq_refl Hmid_sem)
+          as Haff_corr.
+        destruct Haff_corr as [st_src [Hsrc_sem Heq_src]].
+        exists st_src.
+        split; auto.
+        eapply State.eq_trans; eauto.
+      * eapply BaseOpt.affine_opt_prepared_from_poly_correct; eauto.
+    + eapply BaseOpt.affine_opt_prepared_from_poly_correct; eauto.
+  - eapply BaseOpt.affine_opt_prepared_from_poly_correct; eauto.
+Qed.
+
+Lemma phase_diamond_opt_prepared_from_poly_no_iss_band_correct:
+  forall pol st st',
+    PolyLang.wf_pprog_affine pol ->
+    WHEN loop' <- phase_diamond_opt_prepared_from_poly_no_iss_band pol THEN
+    LoopIR.semantics loop' st st' ->
+    exists st'',
+      PolyLang.instance_list_semantics pol st st'' /\
+      State.eq st' st''.
+Proof.
+  intros pol st st' Hwf loop' Hopt Hloop.
+  unfold phase_diamond_opt_prepared_from_poly_no_iss_band in Hopt.
+  destruct (BaseOpt.has_nonscalar_stmt pol) eqn:Hnonscalar.
+  - destruct (BaseOpt.export_for_phase_scheduler pol) as [before_scop|] eqn:Hscop.
+    + eapply try_diamond_phase_pipeline_from_source_pol_band_correct; eauto.
+    + eapply BaseOpt.affine_opt_prepared_from_poly_correct; eauto.
+  - pose proof
+      (PrepareCore.prepared_codegen_correct
+         pol st st' loop' Hopt Hwf Hloop)
+      as Hsem.
+    exists st'. split; auto. apply State.eq_refl.
+Qed.
+
+Definition Opt_prepared_diamond_band := phase_diamond_opt_prepared_band.
+Definition Opt_diamond_band := Opt_prepared_diamond_band.
+
+Theorem Opt_prepared_diamond_band_correct:
+  forall loop st st',
+    WHEN loop' <- Opt_prepared_diamond_band loop THEN
+    LoopIR.semantics loop' st st' ->
+    exists st'',
+      LoopIR.semantics loop st st'' /\
+      State.eq st' st''.
+Proof.
+  intros loop st st' loop' Hopt Hloop.
+  unfold Opt_prepared_diamond_band, phase_diamond_opt_prepared_band in Hopt.
+  bind_imp_destruct Hopt pol0 Hextimp.
+  set (pol := BaseOpt.Strengthen.strengthen_pprog pol0) in *.
+  pose proof Hextimp as Hextok.
+  apply res_to_alarm_correct in Hextok.
+  pose proof
+    (BaseOpt.Strengthen.strengthen_pprog_wf_affine pol0
+       (BaseOpt.extractor_success_wf_pprog_affine loop pol0 Hextok))
+    as Hwf_pol.
+  pose proof
+    (phase_diamond_opt_prepared_from_poly_no_iss_band_correct
+       pol st st' Hwf_pol loop' Hopt Hloop)
+    as Hphase_corr.
+  destruct Hphase_corr as [st_str [Hstr_sem Heq_str]].
+  eapply BaseOpt.Strengthen.instance_list_semantics_unstrengthen in Hstr_sem.
+  pose proof
+    (BaseOpt.Extractor.extractor_correct loop pol0 st st_str Hextok Hstr_sem)
+    as Hext_corr.
+  destruct Hext_corr as [st_src [Hloop_src Heq_src]].
+  exists st_src.
+  split; auto.
+  eapply State.eq_trans.
+  - exact Heq_str.
+  - exact Heq_src.
+Qed.
+
+Theorem Opt_diamond_band_correct:
+  forall loop st st',
+    WHEN loop' <- Opt_diamond_band loop THEN
+    LoopIR.semantics loop' st st' ->
+    exists st'',
+      LoopIR.semantics loop st st'' /\
+      State.eq st' st''.
+Proof.
+  intros.
+  eapply Opt_prepared_diamond_band_correct; eauto.
 Qed.
 
 Theorem Opt_band_correct:
