src/CPolIRs.v
@@ -23,6 +23,8 @@ Module CPolIRs <: POLIRS with Module Instr := CInstr.
    Parameter phase_scop_scheduler: OpenScop -> result (OpenScop * OpenScop).
    Parameter phase_scop_scheduler_with_iss :
      OpenScop -> result (OpenScop * OpenScop).
+   Parameter diamond_phase_scop_scheduler :
+     OpenScop -> result (OpenScop * (OpenScop * OpenScop)).
    Parameter infer_iss_from_source_scop :
      PolyLang.t -> OpenScop -> result (option (PolyLang.t * iss_witness)).
    Parameter infer_tiling_witness_scops:
@@ -47,4 +49,6 @@ Module CPolIRs <: POLIRS with Module Instr := CInstr.
    Definition run_pluto_phase_pipeline := phase_scop_scheduler.
    Definition run_pluto_phase_pipeline_with_iss :=
      phase_scop_scheduler_with_iss.
+   Definition run_pluto_diamond_phase_pipeline :=
+     diamond_phase_scop_scheduler.
 End CPolIRs.
