syntax/SBandTilingOpt.v
@@ -70,6 +70,78 @@ Definition try_phase_pipeline_from_source_pol_band
       end
   end.
 
+Definition try_verified_diamond_after_phase_mid_band
+    (pol_mid: SPolIRs.PolyLang.t)
+    (mid_scop posttile_scop after_scop: OpenScop) : imp SPolIRs.Loop.t :=
+  match SPolOpt.CoreOpt.infer_tiling_witness_scops mid_scop posttile_scop with
+  | Err _ =>
+      SPolOpt.CoreOpt.PrepareCore.prepared_codegen pol_mid
+  | Okk ws =>
+      match SPolOpt.CoreOpt.ValidatorCore.import_canonical_tiled_after_poly pol_mid posttile_scop ws with
+      | Err _ =>
+          SPolOpt.CoreOpt.PrepareCore.prepared_codegen pol_mid
+      | Okk pol_posttile =>
+          BIND ok_shape <- STilingBandSched.checked_tiling_schedule_stripmined_validate_poly pol_mid pol_posttile ws -;
+          if ok_shape then
+            match STilingBandSched.infer_pprog_tiling_bands
+                    (STilingBandSched.outer_to_tiling_pprog pol_mid) ws with
+            | None =>
+                SPolOpt.CoreOpt.PrepareCore.prepared_codegen pol_mid
+            | Some bands =>
+                BIND ok_perm <-
+                  check_pprog_permutable_tiling_bands
+                    (STilingBandSched.outer_to_tiling_pprog pol_mid)
+                    (STilingBandSched.outer_to_tiling_pprog pol_posttile)
+                    ws bands -;
+                if ok_perm then
+                  BIND wf_posttile <- SPolOpt.CoreOpt.ValidatorCore.check_wf_polyprog_general pol_posttile -;
+                  if wf_posttile then
+                    match SPolIRs.PolyLang.from_openscop_schedule_only
+                            pol_posttile after_scop with
+                    | Err _ =>
+                        SPolOpt.CoreOpt.PrepareCore.prepared_codegen pol_mid
+                    | Okk pol_after =>
+                        BIND final_ok <- SPolOpt.CoreOpt.ValidatorCore.validate_general pol_posttile pol_after -;
+                        if final_ok then
+                          BIND wf_after <- SPolOpt.CoreOpt.ValidatorCore.check_wf_polyprog_general pol_after -;
+                          if wf_after then
+                            SPolOpt.CoreOpt.PrepareCore.prepared_codegen
+                              (SPolIRs.PolyLang.current_view_pprog pol_after)
+                          else
+                            SPolOpt.CoreOpt.PrepareCore.prepared_codegen pol_mid
+                        else
+                          SPolOpt.CoreOpt.PrepareCore.prepared_codegen pol_mid
+                    end
+                  else
+                    SPolOpt.CoreOpt.PrepareCore.prepared_codegen pol_mid
+                else
+                  SPolOpt.CoreOpt.PrepareCore.prepared_codegen pol_mid
+            end
+          else
+            SPolOpt.CoreOpt.PrepareCore.prepared_codegen pol_mid
+      end
+  end.
+
+Definition try_diamond_phase_pipeline_from_source_pol_band
+    (pol_source: SPolIRs.PolyLang.t)
+    (before_scop: OpenScop) : imp SPolIRs.Loop.t :=
+  match SPolOpt.CoreOpt.run_pluto_diamond_phase_pipeline before_scop with
+  | Err _ =>
+      SPolOpt.CoreOpt.affine_only_opt_prepared_from_poly pol_source
+  | Okk (mid_scop, (posttile_scop, after_scop)) =>
+      match SPolIRs.PolyLang.from_openscop_like_source pol_source mid_scop with
+      | Err _ =>
+          SPolOpt.CoreOpt.affine_only_opt_prepared_from_poly pol_source
+      | Okk pol_mid =>
+          BIND affine_ok <- SPolOpt.CoreOpt.ValidatorCore.validate pol_source pol_mid -;
+          if affine_ok then
+            try_verified_diamond_after_phase_mid_band
+              pol_mid mid_scop posttile_scop after_scop
+          else
+            SPolOpt.CoreOpt.affine_only_opt_prepared_from_poly pol_source
+      end
+  end.
+
 Definition opt (loop : SPolIRs.Loop.t) : imp SPolIRs.Loop.t :=
   BIND pol0 <- res_to_alarm SPolIRs.PolyLang.dummy (SPolOpt.CoreOpt.Extractor.extractor loop) -;
   let pol := SPolOpt.CoreOpt.Strengthen.strengthen_pprog pol0 in
@@ -86,8 +158,24 @@ Definition opt (loop : SPolIRs.Loop.t) : imp SPolIRs.Loop.t :=
   else
     SPolOpt.CoreOpt.PrepareCore.prepared_codegen pol.
 
+Definition opt_diamond (loop : SPolIRs.Loop.t) : imp SPolIRs.Loop.t :=
+  BIND pol0 <- res_to_alarm SPolIRs.PolyLang.dummy (SPolOpt.CoreOpt.Extractor.extractor loop) -;
+  let pol := SPolOpt.CoreOpt.Strengthen.strengthen_pprog pol0 in
+  if SPolOpt.CoreOpt.has_nonscalar_stmt pol then
+    match SPolOpt.CoreOpt.export_for_phase_scheduler pol with
+    | Some before_scop =>
+        try_diamond_phase_pipeline_from_source_pol_band pol before_scop
+    | None =>
+        SPolOpt.CoreOpt.affine_only_opt_prepared_from_poly pol
+    end
+  else
+    SPolOpt.CoreOpt.PrepareCore.prepared_codegen pol.
+
 Definition opt_prepared (loop : SPolIRs.Loop.t) : imp SPolIRs.Loop.t :=
   opt loop.
+
+Definition opt_diamond_prepared (loop : SPolIRs.Loop.t) : imp SPolIRs.Loop.t :=
+  opt_diamond loop.
 
 Definition opt_poly (pol : SPolIRs.PolyLang.t) : imp SPolIRs.Loop.t :=
   let pol' := SPolOpt.CoreOpt.Strengthen.strengthen_pprog pol in
@@ -104,8 +192,26 @@ Definition opt_poly (pol : SPolIRs.PolyLang.t) : imp SPolIRs.Loop.t :=
   else
     SPolOpt.CoreOpt.PrepareCore.prepared_codegen pol'.
 
+Definition opt_diamond_poly (pol : SPolIRs.PolyLang.t) : imp SPolIRs.Loop.t :=
+  let pol' := SPolOpt.CoreOpt.Strengthen.strengthen_pprog pol in
+  if SPolOpt.CoreOpt.has_nonscalar_stmt pol' then
+    match SPolOpt.CoreOpt.export_for_phase_scheduler pol' with
+    | Some before_scop =>
+        try_diamond_phase_pipeline_from_source_pol_band pol' before_scop
+    | None =>
+        SPolOpt.CoreOpt.affine_only_opt_prepared_from_poly pol'
+    end
+  else
+    SPolOpt.CoreOpt.PrepareCore.prepared_codegen pol'.
+
 Definition opt_scop (scop : OpenScop) : imp SPolIRs.Loop.t :=
   match SPolIRs.PolyLang.from_openscop_complete scop with
   | Okk pol => opt_poly pol
+  | Err msg => res_to_alarm SPolIRs.Loop.dummy (Err msg)
+  end.
+
+Definition opt_diamond_scop (scop : OpenScop) : imp SPolIRs.Loop.t :=
+  match SPolIRs.PolyLang.from_openscop_complete scop with
+  | Okk pol => opt_diamond_poly pol
   | Err msg => res_to_alarm SPolIRs.Loop.dummy (Err msg)
   end.
